@prefix manifest: <https://somanyaircraft.com/data/schema/manifest#> .
@prefix dcat: <http://www.w3.org/ns/dcat#> .
@prefix sh: <http://www.w3.org/ns/shacl#> .
@prefix skos: <http://www.w3.org/2004/02/skos/core#> .
@prefix rdfs: <http://www.w3.org/2000/01/rdf-schema#> .
@prefix owl: <http://www.w3.org/2002/07/owl#> .
@prefix xsd: <http://www.w3.org/2001/XMLSchema#> .
@prefix dcterms: <http://purl.org/dc/terms/> .
@prefix sma: <https://somanyaircraft.com/data/schema/core#> .

manifest: a owl:Ontology ;
	dcterms:title "SMA Data Manifest Ontology" ;
	owl:versionInfo "version 1; 2025-10-12" ;
	dcterms:publisher <https://somanyaircraft.com> .

manifest:alternateNamespace a owl:ObjectProperty ;
	rdfs:label "alternate namespace" ;
	rdfs:comment "Used to provide an alternate namespace URI, to be used at the manifest processor's discretion." ;
	rdfs:domain sh:PrefixDeclaration ;
	rdfs:range rdfs:Resource .

manifest:Directory a dcterms:MediaType ;
	rdfs:comment "Used as a value for dcat:mediaType to indicate that the distribution is a directory." .

manifest:mapping a owl:ObjectProperty ;
	rdfs:label "RML/R2RML mapping" ;
	rdfs:comment "Provides the RML or R2RML mapping that is applied to the distribution before loading." ;
	rdfs:domain dcat:Distribution ;
	rdfs:range rdfs:Resource .

manifest:context a owl:ObjectProperty ;
	rdfs:label "JSON-LD context" ;
	rdfs:comment "Provides the JSON-LD context that is applied to the distribution when loading it." ;
	rdfs:domain dcat:Distribution ;
	rdfs:range rdfs:Resource .

manifest:SourceTypes a skos:ConceptScheme .

manifest:OntologySource a skos:Concept ;
	skos:inScheme manifest:Sourcetypes .

manifest:DataSource a skos:Concept ;
	skos:inScheme manifest:SourceTypes .

manifest:UncategorizedSource a skos:Concept ;
	skos:inScheme manifest:SourceTypes .
